labs/DenotationalSemantics/Denotational.v
@@ -1,0 +1,1106 @@
+From PLF Require Import Imp.
+From PLF Require Import Maps.
+From DS Require Import Fixpoints.
+From Coq Require Import Lia.
+From Coq Require Import Setoid.
+
+Definition AExpDom := PSet (nat * state).
+Definition BExpDom := PSet (bool * state).
+Definition ComDom := PSet (state * state).
+
+Reserved Notation "'[[' a ']]A'" (at level 40).
+Reserved Notation "'[[' b ']]B'" (at level 40).
+Reserved Notation "'[[' c ']]'" (at level 40).
+
+Declare Scope denote_scope.
+
+Notation "{{ v | P }}" := (fun v => P) (v pattern) : denote_scope.
+
+Open Scope denote_scope.
+
+(* ====== Denotational Semantics of Arithmetic Expressions ======= *)
+
+(* The semantic domain for arithmetic expressions is pairs of states
+   and numbers: *)
+
+(* ⟦n⟧A ≡ {(σ, n)}
+   ⟦x⟧A ≡ {(σ, σ(x))}
+   ⟦a1+a2⟧A ≡ {(σ, n + m) | (σ, n) ∈ ⟦a1⟧A ∧ (σ, m) ∈ ⟦a2⟧A}
+   ⟦a1-a2⟧A ≡ {(σ, n - m) | (σ, n) ∈ ⟦a1⟧A  ∧ (σ, m) ∈ ⟦a2⟧A}
+   ⟦a1*a2⟧A ≡ {(σ, n * m) | (σ, n) ∈ ⟦a1⟧A  ∧ (σ, m) ∈ ⟦a2⟧A} *)
+Fixpoint denote_A (a : aexp) : AExpDom :=
+  match a with
+  | ANum n => {{ ( m, st ) | m = n }}
+
+  (* ⟦x⟧A ≡ {(σ, σ(x))} *)
+  | AId x  => {{ ( m, st ) |  m = st x }}
+
+  (* ⟦a1+a2⟧A ≡ {(σ, n + m) | (σ, n) ∈ ⟦a1⟧A ∧ (σ, m) ∈ ⟦a2⟧A} *)
+  | <{a1 + a2}> => {{ (n', st) |
+                      exists v1 v2,
+                      (v1, st) ∈ [[ a1 ]]A
+                      /\ (v2, st) ∈ [[ a2 ]]A
+                      /\ n' = v1 + v2 }}
+
+  (* ⟦a1-a2⟧A ≡ {(σ, n - m) | (σ, n) ∈ ⟦a1⟧A  ∧ (σ, m) ∈ ⟦a2⟧A} *)
+  | <{a1 - a2}> => {{ (n', st) |
+                      exists v1 v2,
+                      (v1, st) ∈ [[ a1 ]]A
+                      /\ (v2, st) ∈ [[ a2 ]]A
+                      /\ n' = v1 - v2 }}
+
+  (* ⟦a1*a2⟧A ≡ {(σ, n * m) | (σ, n) ∈ ⟦a1⟧A  ∧ (σ, m) ∈ ⟦a2⟧A} *)
+  | <{a1 * a2}> => {{ (n', st) |
+                      exists v1 v2,
+                      (v1, st) ∈ [[ a1 ]]A
+                      /\ (v2, st) ∈ [[ a2 ]]A
+                      /\ n' = v1 * v2 }}
+  end
+where "'[[' a ']]A'" := (denote_A a).
+
+(* We can already state and prove some interesting properties about
+   our denotation function!
+
+   Firstly, there exists (at most) one corresponding value for each
+   state in the denotation of an expression. This captures a notion of
+   determinism for an expression. *)
+Theorem aexp_eqv_unique :
+  forall (a : aexp)
+         (m n : nat)
+         (st : state),
+    (m, st) ∈ ([[a ]]A) ->
+    (n, st) ∈ ([[a ]]A) ->
+    m = n.
+Proof.
+  induction a; simpl; intros.
+  - In_inversion. subst. reflexivity.
+  - In_inversion. subst. reflexivity.
+  - In_inversion. subst.
+    erewrite IHa1 with (m := x1) (n := x), IHa2 with (m := x0) (n := x2) by
+      eassumption.
+    reflexivity.
+  - In_inversion. subst.
+    erewrite IHa1 with (m := x1) (n := x), IHa2 with (m := x0) (n := x2) by
+      eassumption.
+    reflexivity.
+  - In_inversion. subst.
+    erewrite IHa1 with (m := x1) (n := x), IHa2 with (m := x0) (n := x2) by
+      eassumption.
+    reflexivity.
+Qed.
+
+(* Secondly, there exists exactly one corresponding value for each
+   state in the denotation of an expression. *)
+Theorem denote_aexp_defined :
+  forall (a : aexp) (st : state),
+  exists n, (n, st) ∈ [[a]]A.
+Proof.
+  intros; induction a.
+  - exists n; In_intro; simpl; reflexivity.
+  - eexists (st x); In_intro; simpl; reflexivity.
+  - destruct IHa1 as [n denote_a1].
+    destruct IHa2 as [m denote_a2].
+    exists (n + m); In_intro; simpl; eexists _, _; repeat split; assumption.
+  - destruct IHa1 as [n denote_a1].
+    destruct IHa2 as [m denote_a2].
+    exists (n - m); In_intro; simpl; eexists _, _; repeat split; assumption.
+  - destruct IHa1 as [n denote_a1].
+    destruct IHa2 as [m denote_a2].
+    exists (n * m); In_intro; simpl; eexists _, _; repeat split; assumption.
+Qed.
+
+(* Two expressions are semantically equivalent if their denotation is
+   the same set of states and values. *)
+Definition aexp_eqv (a a' : aexp) : Prop :=
+  Same_set ([[ a ]]A) ([[ a' ]]A).
+
+Notation "a1 '==A' a2 " := (aexp_eqv a1 a2) (at level 40).
+
+(* Since expression equivalence is defined in terms of set
+   equivalence, we can obtain proofs that it is reflexive,
+   transititve, and symmetric for 'free'. *)
+Lemma aexp_eqv_refl : forall (a : aexp),
+    a ==A a.
+Proof. intro; apply Same_set_refl. Qed.
+
+Lemma aexp_eqv_sym : forall (a1 a2 : aexp),
+    a1 ==A a2 -> a2 ==A a1.
+Proof. intros; apply Same_set_sym; assumption. Qed.
+
+Lemma aexp_eqv_trans : forall (a1 a2 a3 : aexp),
+    a1 ==A a2 -> a2 ==A a3 -> a1 ==A a3.
+Proof. intros; eapply Same_set_trans; eassumption. Qed.
+
+(* We can use the following command to register the fact that our
+   notion of equivalence for arithmetic expressions is actually an
+   equivalence relation. This allows us to use the [reflexivity],
+   [symmetry], and [transitivity] tactics with goals and assumptions
+   about arithmetic equivalence, just as we can with regular
+   equality. *)
+Add Parametric Relation : aexp aexp_eqv
+    reflexivity  proved by aexp_eqv_refl
+    symmetry proved by aexp_eqv_sym
+    transitivity proved by aexp_eqv_trans
+    as eqv_aexp_eqv.
+
+Example aexp_tactic_ex : forall (a1 a2 a3 : aexp),
+    a1 ==A a2 -> a3 ==A a2 -> a1 ==A a3.
+Proof.
+  intros.
+  symmetry in H.
+  symmetry.
+  transitivity a2.
+  assumption.
+  assumption.
+Qed.
+
+(* We can reason about equivalence of two expressions by reasoning
+   about their denotations, allowing us to use any lemmas or theorems
+   about sets. *)
+Example aexp_eqv_example: <{ X + Y }> ==A <{ Y + X }>.
+Proof.
+  (* To show two expressions are equivalent, we need to prove their
+  denotations are the same. That is, we need to show that every
+  element in the denotation of [X + Y] is included in [Y + X] and vice
+  versa. *)
+  split; intros (n, st) In_st.
+  - (* In the first case, we need to show that
+       (n, st) ∈ [[X + Y]]A implies  (n, st) ∈ [[Y + X]]A *)
+  (* [In_inversion] is a custom tactic for working with assumptions
+     about memembership in a set. It is defined in Fixpoints.v *)
+    simpl in In_st. In_inversion. subst.
+    (* [In_intro] is a custom tactic for working with goals about set
+       memembership, it is also defined in Fixpoints.v *)
+    simpl. In_intro.
+    exists (st Y), (st X); repeat split. lia.
+  - (* In the second case, we need to show that
+       (n, st) ∈ [[Y + X]]A implies  (n, st) ∈ [[X + Y]]A *)
+    simpl in In_st. In_inversion.
+    In_intro.
+    eexists (st X), (st Y); repeat split.
+    lia.
+Qed.
+
+Example aexp_eqv_example_2 :
+  forall (a : aexp), <{ 0 + a }> ==A <{ a }>.
+Proof.
+  split; simpl; intros (n, st) In_st.
+  - In_inversion. subst. assumption.
+  - In_inversion.
+    In_intro.
+    eexists _, _; repeat split; try assumption.
+Qed.
+
+Example aexp_eqv_example_3 :
+  forall (a : aexp), <{ a - a }> ==A <{ 0 }>.
+Proof.
+  split; simpl; intros (n, st) In_st.
+  - In_inversion. subst.
+    erewrite aexp_eqv_unique with (m := x) (n := x0) by eassumption.
+    In_intro; lia.
+  - In_inversion.
+    In_intro.
+    destruct (denote_aexp_defined a st) as [m denote_a].
+    exists m, m; repeat split; try assumption.
+    lia.
+Qed.
+
+(* Semantic equivalence gives us a natural specification of the
+   correctness of a program transformation: *)
+Fixpoint aexp_opt_zero (a : aexp) : aexp :=
+match a with
+| ANum n => ANum n
+| AId X => AId X
+| APlus (ANum 0) e2 => aexp_opt_zero e2
+| APlus e1 e2 => APlus (aexp_opt_zero e1) (aexp_opt_zero e2)
+| AMinus e1 e2 => AMinus (aexp_opt_zero e1) (aexp_opt_zero e2)
+| AMult e1 e2 => AMult (aexp_opt_zero e1) (aexp_opt_zero e2)
+end.
+
+Theorem aexp_opt_zero_sound
+  : forall a, aexp_opt_zero a ==A a.
+Proof.
+  (* New *tactical* alert: *)
+  induction a; simpl; try reflexivity.
+  (* - reflexivity.
+  - reflexivity. *)
+  - (* We could proceed by case analysis on [a1], but this is a golden
+    opportunity to explore Coq's support for equational reasoning with
+    equivalences like aexp_eqv. *)
+Abort.
+
+(* The semantics of arithemetic expressions is /compositional/: the
+   meaning of an expression is derived from meaning of its
+   subexpressions. We can exploit this property to show that
+   expression equivalence is a /congruence/: that two expressions are
+   equivalent if their subexpressions are equivalent.  *)
+Lemma plus_eqv_cong : forall a1 a2 a1' a2',
+    a1 ==A a1' ->
+    a2 ==A a2' ->
+    <{a1 + a2}> ==A <{a1' + a2'}>.
+Proof.
+  intros a1 a2 a1' a2' a1_eqv a2_eqv.
+  split; intros (a, st) v_In.
+  - (* Since [[a1 + a2]]A and [[a1' + a2']]A are built from the
+       results of [[a1]]A, [[a2]]A, [[a1']]A, and [[a2]]A, their
+       equivalence follows from the assumptions that [[a1]]A and
+       [[a2]]A are equivalent to [[a1']]A [[a2']]A *)
+    simpl in *; In_inversion; In_intro.
+    exists x, x0.
+    repeat split; try tauto.
+    + apply a1_eqv; assumption.
+    + apply a2_eqv; assumption.
+  - simpl in *; In_inversion; In_intro.
+    exists x, x0.
+    repeat split; try tauto.
+    + apply a1_eqv; assumption.
+    + apply a2_eqv; assumption.
+Qed.
+
+(* It turns out that Coq includes built in support for a generalized
+   form of rewriting using equivalence relations. In order for
+   rewriting to work however, we have to demonstrate which cases they
+   work in. This amounts to proving congruences like the lemma above,
+   but we also have to use a specialized Command to let Coq know that
+   we're extending the behavior of the [rewrite] tactic.
+
+   The 'Generalized Rewriting' chapter of Coq's documentation has the
+   full details on all the bells and whistles of this feature, but
+   we'll just give a taste of how this works here. *)
+
+Add Parametric Morphism : APlus
+    with signature aexp_eqv ==> aexp_eqv ==> aexp_eqv
+      as plus_eqv_cong'.
+Proof.
+  intros. apply plus_eqv_cong; assumption.
+Qed.
+
+(* We can skip the process by proving the desired congruence fact
+   directly: *)
+(* Lemma minus_eqv_cong : forall a1 a2 a1' a2',
+    a1 ==A a1' ->
+    a2 ==A a2' ->
+    <{a1 - a2}> ==A <{a1' - a2'}>.
+Proof. *)
+
+Add Parametric Morphism : AMinus
+    with signature aexp_eqv ==> aexp_eqv ==> aexp_eqv
+      as minus_eqv_cong.
+Proof.
+  intros a1 a1' a1_eqv a2 a2' a2_eqv; split;
+    simpl; intros (a, st) v_In; In_inversion.
+  - In_intro.
+    exists x, x0.
+    repeat split; try tauto.
+    + apply a1_eqv; assumption.
+    + apply a2_eqv; assumption.
+  - In_intro.
+    exists x, x0.
+    repeat split; try tauto.
+    + apply a1_eqv; assumption.
+    + apply a2_eqv; assumption.
+Qed.
+
+(* Lemma mult_eqv_cong : forall a1 a2 a1' a2',
+    a1 ==A a1' ->
+    a2 ==A a2' ->
+    <{a1 * a2}> ==A <{a1' * a2'}>. *)
+Add Parametric Morphism : AMult
+    with signature aexp_eqv ==> aexp_eqv ==> aexp_eqv
+      as mult_eqv_cong.
+Proof.
+  intros a1 a1' a1_eqv a2 a2' a2_eqv; split;
+    simpl; intros (a, st) v_In; In_inversion.
+  - In_intro.
+    exists x, x0.
+    repeat split; try tauto.
+    + apply a1_eqv; assumption.
+    + apply a2_eqv; assumption.
+  - In_intro.
+    exists x, x0.
+    repeat split; try tauto.
+    + apply a1_eqv; assumption.
+    + apply a2_eqv; assumption.
+Qed.
+
+Theorem aexp_opt_zero_sound
+  : forall a, aexp_opt_zero a ==A a.
+Proof.
+  induction a; simpl; try reflexivity.
+  - (* Having done all this work, our standard rewrite tactics now
+    work with assumptions and goals involving ==A! *)
+    rewrite <- IHa1 at 2.
+    rewrite <- IHa2.
+    destruct a1; simpl; try reflexivity.
+    destruct n; try reflexivity.
+    rewrite aexp_eqv_example_2.
+    reflexivity.
+  - rewrite IHa1, IHa2. reflexivity.
+  - rewrite IHa1, IHa2. reflexivity.
+Qed.
+
+(* ====== Denotational Semantics of Boolean Expressions ======= *)
+
+(* The semantic domain for boolean expressions is pairs of states
+   and booleans:
+
+   ⟦true⟧B ≡ {(σ, true)}
+   ⟦false⟧B ≡ {(σ, false)}
+   ⟦a1 == a2⟧B ≡ {(σ, n =? m) | (σ, n) ∈ ⟦a1⟧B ∧ (σ, m) ∈ ⟦a2⟧B}
+   ⟦a1 <= a2⟧B ≡ {(σ, n <=? m) | (σ, n) ∈ ⟦a1⟧B  ∧ (σ, m) ∈ ⟦a2⟧B}
+   ⟦b1 && b2⟧B ≡ {(σ, v1 && v2) | (σ, v1) ∈ ⟦b1⟧B  ∧ (σ, v2) ∈ ⟦b2⟧B} *)
+Fixpoint denote_B (b : bexp) : BExpDom :=
+  match b with
+  | <{true}> => {{ (v, st) | v = true }}
+
+  | <{false}> => {{ (v, st) | v = false }}
+
+  | <{a1 = a2}> => {{ (v, st) |
+    exists v1 v2,
+    (v1, st) ∈ [[ a1 ]]A /\ (v2, st) ∈ [[ a2 ]]A
+    /\ (v1 = v2 <-> v = true)}}
+
+  | <{ a1 <= a2}> => {{ (v, st) |
+    exists v1 v2,
+    (v1, st) ∈ [[ a1 ]]A /\ (v2, st) ∈ [[ a2 ]]A
+    /\ (v1 <= v2 <-> v = true) }}
+
+  | <{~ b1}> => {{ (v, st) |  (negb v, st) ∈ [[ b1 ]]B }}
+
+  | <{b1 && b2}> => {{ (v, st) |
+    exists v1 v2,
+    (v1, st) ∈ [[ b1 ]]B /\ (v2, st) ∈ [[ b2 ]]B
+    /\ v = (andb v1 v2) }}
+
+  (* Uncomment to account for larger set of boolean expressions in SF. *)
+
+  (* | <{a1 <> a2}> => {{ (v, st) |
+    exists v1 v2,
+    (v1, st) ∈ [[ a1 ]]A /\ (v2, st) ∈ [[ a2 ]]A
+    /\ (v1 = v2 <-> v = false) }}
+
+  | <{ a1 > a2}> => {{ (v, st) |
+    exists v1 v2,
+    (v1, st) ∈ [[ a1 ]]A /\ (v2, st) ∈ [[ a2 ]]A
+    /\ (v1 > v2 <-> v = true) }} *)
+
+
+  end
+where "'[[' b ']]B'" := (denote_B b).
+
+Definition bexp_eqv (b b' : bexp) : Prop :=
+  Same_set ([[ b ]]B) ([[ b' ]]B).
+
+Notation "b1 '==B' b2 " := (bexp_eqv b1 b2) (at level 40).
+
+Lemma bexp_eqv_refl : forall (b : bexp),
+    b ==B b.
+Proof. intro; apply Same_set_refl. Qed.
+
+Lemma bexp_eqv_sym : forall (b1 b2 : bexp),
+    b1 ==B b2 -> b2 ==B b1.
+Proof. intros; apply Same_set_sym; assumption. Qed.
+
+Lemma bexp_eqv_trans : forall (b1 b2 b3 : bexp),
+    b1 ==B b2 -> b2 ==B b3 -> b1 ==B b3.
+Proof. intros; eapply Same_set_trans; eassumption. Qed.
+
+Add Parametric Relation : bexp bexp_eqv
+    reflexivity proved by bexp_eqv_refl
+    symmetry proved by bexp_eqv_sym
+    transitivity proved by bexp_eqv_trans
+    as eqv_bexp_eqv.
+
+Theorem beq_eqv_example : forall a, <{ a = a }> ==B <{ true }>.
+Proof.
+  split; simpl; intros (n, st) In_st.
+  - In_inversion.
+    erewrite aexp_eqv_unique with (m := x) (n := x0) in H1 by eassumption.
+    rewrite <- H1.
+    reflexivity.
+  - In_inversion.
+    In_intro.
+    destruct (denote_aexp_defined a st) as [m denote_a].
+    exists m, m; repeat split; try assumption.
+    subst; reflexivity.
+Qed.
+
+(* We can once again prove some congrence facts about the
+   compositionality of equivalence of boolean expressions: *)
+
+(*Lemma beq_eqv_cong : forall a1 a2 a1' a2',
+    a1 ==A a1' ->
+    a2 ==A a2' ->
+    <{a1 = a2}> ==B <{a1' = a2'}>. *)
+Add Parametric Morphism : BEq
+    with signature aexp_eqv ==> aexp_eqv ==> bexp_eqv
+      as beq_eqv_cong.
+Proof.
+  intros a1 a1' a1_eqv a2 a2' a2_eqv.
+  split; intros (b, st) v_In.
+  - simpl in *; In_inversion; In_intro.
+    exists x, x0.
+    repeat split; try tauto.
+    + apply a1_eqv; assumption.
+    + apply a2_eqv; assumption.
+  - simpl in *; In_inversion; In_intro.
+    exists x, x0.
+    repeat split; try tauto.
+    + apply a1_eqv; assumption.
+    + apply a2_eqv; assumption.
+Qed.
+
+(* Lemma ble_eqv_cong : forall a1 a2 a1' a2',
+    a1 ==A a1' ->
+    a2 ==A a2' ->
+    <{a1 <= a2}> ==B <{a1' <= a2'}>. *)
+Add Parametric Morphism : BLe
+    with signature aexp_eqv ==> aexp_eqv ==> bexp_eqv
+      as ble_eqv_cong.
+Proof.
+  intros a1 a1' a1_eqv a2 a2' a2_eqv; split;
+    simpl; intros (b, st) v_In; In_inversion.
+  - In_intro.
+    exists x, x0.
+    repeat split; try tauto.
+    + apply a1_eqv; assumption.
+    + apply a2_eqv; assumption.
+  - In_intro.
+    exists x, x0.
+    repeat split; try tauto.
+    + apply a1_eqv; assumption.
+    + apply a2_eqv; assumption.
+Qed.
+
+(* Lemma bnot_eqv_cong : forall b1 b1',
+    b1 ==B b1' ->
+    <{~ b1}> ==B <{~ b1'}>. *)
+Add Parametric Morphism : BNot
+    with signature bexp_eqv ==> bexp_eqv
+      as bnot_eqv_cong.
+Proof.
+  intros b1 b1' b1_eqv; split;
+    simpl; intros (b, st) v_In; In_inversion.
+  - In_intro. apply b1_eqv; assumption.
+  - In_intro. apply b1_eqv; assumption.
+Qed.
+
+(* Lemma band_eqv_cong : forall b1 b2 b1' b2',
+    b1 ==B b1' ->
+    b2 ==B b2' ->
+    <{b1 && b2}> ==B <{b1' && b2'}>. *)
+Add Parametric Morphism : BAnd
+    with signature bexp_eqv ==> bexp_eqv ==> bexp_eqv
+      as band_eqv_cong.
+Proof.
+  intros b1 b1' b1_eqv b2 b2' b2_eqv; split;
+    simpl; intros (b, st) v_In; In_inversion.
+  - In_intro.
+    exists x, x0; repeat split; try assumption.
+    apply b1_eqv; assumption.
+    apply b2_eqv; assumption.
+  - In_intro.
+    exists x, x0; repeat split; try assumption.
+    apply b1_eqv; assumption.
+    apply b2_eqv; assumption.
+Qed.
+
+(* These congruence facts are quite useful for reasoning about
+   particular expressions. We could apply these lemmas directly, as in
+   this proof: *)
+Theorem bexp_eqv_example: <{ X - X = 0 }> ==B <{ true }>.
+Proof.
+  (* We first use the fact that equivalence (i.e. set equality) is
+  transitive to simplify the left-hand side of the equality. *)
+  eapply bexp_eqv_trans with (b2 := <{0 = 0}>).
+  - apply beq_eqv_cong.
+    + apply aexp_eqv_example_3.
+    + reflexivity.
+  - split; simpl; intros (b, st) v_In; In_inversion; In_intro; subst.
+    + apply H1; reflexivity.
+    + exists 0, 0; repeat split.
+Qed.
+
+(* Thanks to the special commands we used above, though, we can also
+   use the rewrite tactic to prove such examples directly: *)
+Theorem bexp_eqv_example': <{ X - X = 0 }> ==B <{ true }>.
+Proof.
+  intros.
+  rewrite aexp_eqv_example_3.
+  rewrite beq_eqv_example.
+  reflexivity.
+Qed.
+
+(* ======== Denotational Semantics of Imp Commands ========= *)
+
+(* The semantic domain for commands is pairs of initial and final
+   states: *)
+
+(*⟦skip⟧C ≡ {(σ, σ)}
+  ⟦x:=a⟧C ≡ {(σ, [x↦v]σ) | (σ, v) ∈ ⟦a⟧A }
+  ⟦c1;c2⟧C ≡ {(σ1, σ3) | ∃σ2.    (σ1, σ2) ∈ ⟦c1⟧c
+                                     ⋀ (σ2, σ3) ∈ ⟦c2⟧c}
+  ⟦if b then ct else ce⟧C ≡
+     {(σ1, σ2) | (σ1, true) ∈ ⟦eB⟧B ⋀ (σ1, σ2) ∈ ⟦ct⟧C }
+   ∪ {(σ1, σ2) | (σ1, false) ∈ ⟦eB⟧B ⋀ (σ1, σ2) ∈ ⟦ce⟧C}
+
+  ⟦while b do c end⟧C ≡ LFP F
+
+  where
+  F(rec) = {(σ, σ) | (σ, false) ∈ ⟦b⟧B}
+           ∪ {(σ1, σ3) | (σ1, true) ∈ ⟦b⟧B
+                              ∧ ∃σ2. (σ1, σ2) ∈ ⟦c⟧c
+                                      ⋀ (σ2, σ3) ∈ rec} *)
+
+(*The denotation of while loops uses the least fixed point [LFP]
+  combinator defined in Fixpoints.v. *)
+Fixpoint denote_Com (c : com)
+  : ComDom :=
+  match c with
+  | <{ skip }> =>
+    {{ (st, st') | st = st' }}
+  | <{x := a1}> => {{ (st, st') | exists v,
+                               (v, st) ∈ [[a1]]A
+                               /\ st' = t_update st x v }}
+
+  | <{c1; c2}> => {{ (st, st') |
+                   exists st'',
+                   (st, st'') ∈ [[c1]] /\
+                   (st'', st') ∈ [[c2]] }}
+
+  | <{ if b then c1 else c2 end }> =>
+    {{ (st, st') |
+      ((true, st) ∈ [[b]]B /\ (st, st') ∈ [[c1]])
+      \/ ((false, st) ∈ [[b]]B /\ (st, st') ∈ [[c2]]) }}
+
+  | <{ while b do c end }> =>
+    LFP (fun (phi : PSet _) =>
+           {{ (st, st') |
+              ((false, st) ∈ [[b]]B /\ st' = st)
+               \/ (exists st'',
+                      (true, st) ∈ [[b]]B /\
+                      (st, st'') ∈ [[c]]
+                      /\  (st'', st') ∈ phi) }})
+
+
+  end
+where "'[[' c ']]'" := (denote_Com c).
+
+(* Two commands are semantically equivalent if their denotation is the
+   same set of starting and final states. *)
+
+Definition com_eqv (c c' : com) : Prop :=
+  Same_set ([[ c ]]) ([[c']]).
+
+Notation "c1 '==C' c2 " := (com_eqv c1 c2) (at level 40).
+
+Lemma com_eqv_refl : forall (c : com),
+    c ==C c.
+Proof. intro; apply Same_set_refl. Qed.
+
+Lemma com_eqv_sym : forall (c1 c2 : com),
+    c1 ==C c2 -> c2 ==C c1.
+Proof. intros; apply Same_set_sym; assumption. Qed.
+
+Lemma com_eqv_trans : forall (c1 c2 c3 : com),
+    c1 ==C c2 -> c2 ==C c3 -> c1 ==C c3.
+Proof. intros; eapply Same_set_trans; eassumption. Qed.
+
+Add Parametric Relation : com com_eqv
+    reflexivity proved by com_eqv_refl
+    symmetry proved by com_eqv_sym
+    transitivity proved by com_eqv_trans
+    as eqv_com_eqv.
+
+(* We can again show that command equivalence is a /congruence/: that two
+   programs are equivalent if their subterms are equivalent.
+
+   The first step is to show this holds for individual commands.
+
+Lemma seq_eq_cong : forall c1 c2 c1' c2',
+    c1 ==C c1' ->
+    c2 ==C c2' ->
+    <{c1; c2}> ==C <{c1'; c2'}>. *)
+Add Parametric Morphism : CSeq
+    with signature com_eqv ==> com_eqv ==> com_eqv
+      as seq_eq_cong.
+Proof.
+  intros; split; simpl; intros (st, st') X_In; In_inversion.
+  - exists x1; split.
+    + apply H; assumption.
+    + apply H0; assumption.
+  - exists x1; split.
+    + apply H; assumption.
+    + apply H0; assumption.
+Qed.
+
+(* Lemma if_eq_cong : forall b c1 c2 c1' c2',
+    c1 ==C c1' ->
+    c2 ==C c2' ->
+    <{if b then c1 else c2 end}> ==C <{if b then c1' else c2' end}>. *)
+Add Parametric Morphism : CIf
+    with signature bexp_eqv ==> com_eqv ==> com_eqv ==> com_eqv
+      as if_eq_cong.
+Proof.
+  intros; split; simpl; intros ? X_In; In_inversion.
+  - left; intuition.
+    + apply H. assumption.
+    + apply H0. assumption.
+  - right; intuition.
+    + apply H. assumption.
+    + apply H1. assumption.
+  - left; intuition.
+    + apply H. assumption.
+    + apply H0. assumption.
+  - right; intuition.
+    + apply H. assumption.
+    + apply H1. assumption.
+Qed.
+
+(* To show that LFP is a proper fixed point in subsequent proofs, we
+   need to show that if is applied to a monotone function. *)
+Lemma while_body_monotone :
+  forall b c,
+    Monotone (fun (phi : PSet _) =>
+           {{ (st, st') |
+              ((false, st) ∈ [[b]]B /\ st' = st)
+               \/ (exists st'',
+                      (true, st) ∈ [[b]]B /\
+                      (st, st'') ∈ [[c]]
+                      /\  (st'', st') ∈ phi) }}).
+Proof.
+  unfold Monotone, Subset; intros.
+  In_inversion.
+  - In_intro. subst; left; split; try assumption; reflexivity.
+  - right; eexists _; intuition; try eassumption.
+    apply H; eassumption.
+Qed.
+
+(* Lemma while_eq_cong : forall b c1 c1',
+    c1 ==C c1' ->
+    <{while b do c1 end}> ==C <{while b do c1' end}>. *)
+Add Parametric Morphism : CWhile
+    with signature bexp_eqv ==> com_eqv ==> com_eqv
+      as while_eq_cong.
+Proof.
+  intros; split; simpl; intros ? X_In; In_inversion.
+  - intuition.
+    + eapply Ind in X_In.
+      apply X_In.
+      unfold FClosed.
+      intros ? ?.
+      In_inversion.
+      intuition; subst.
+      * apply LFP_fold.
+        apply while_body_monotone.
+        left; intuition.
+        apply H; assumption.
+      * apply LFP_fold.
+        apply while_body_monotone.
+        right. exists x1; intuition.
+        -- apply H; assumption.
+        -- apply H0; assumption.
+  - intuition.
+    + eapply Ind in X_In.
+      apply X_In.
+      unfold FClosed.
+      intros ? ?.
+      In_inversion.
+      intuition; subst.
+      * apply LFP_fold.
+        apply while_body_monotone.
+        left; intuition.
+        apply H; assumption.
+      * apply LFP_fold.
+        apply while_body_monotone.
+        right.
+        exists x1; intuition.
+        -- apply H; assumption.
+        -- apply H0; assumption.
+Qed.
+
+(* Using the denotational semantics of commands, we can prove that
+   programs have the same meaning: *)
+Lemma seq_skip_opt :
+  forall c,
+    <{skip; c}> ==C c.
+Proof.
+  intros c; split; intros (st, st') In_st.
+  - (* (st, st') ∈ [[skip; c]] -> (st, st') ∈ [[c]] *)
+    simpl in *; In_inversion.
+    subst.
+    In_intro; assumption.
+  - (* (st, st') ∈ [[c]] -> (st, st') ∈ [[skip; c]] *)
+    (* In this case, we need to show that (st, st') ∈ [[skip; c]] by
+       giving an intermediate state [st''], such that (st, st'') ∈
+       [[skip]] and (st'', st') ∈ [[c]]. Since [[skip]] only contains
+       pairs of the same state, the state [st] fits the bill.  *)
+    simpl in *. In_intro.
+    exists st; split.
+    + reflexivity.
+    + assumption.
+Qed.
+
+(* Using the denotational semantics of commands, we can show that if
+   the condition of an if expression is equivalent to true, the entire
+   expression is semantically equivalent to the then branch: *)
+Theorem if_true: forall b c1 c2,
+    b ==B <{true}>  ->
+    <{ if b then c1 else c2 end }> ==C  c1.
+Proof.
+  intros b c1 c2 Hb.
+  split; intros (st, st') st_In.
+  - (* We need to show that (st, st') ∈ [[<{ if b then c1 else c2 end }>]]
+       implies (st, st') ∈ [[c1]] *)
+    (* By simplifying [[<{ if b then c1 else c2 end }>]], we can do
+       case analysis on what must be true of (st, st') if it is a
+       member of that set. *)
+    simpl in st_In; In_inversion.
+    + (* In particular, either ([[b ]]B) ∈ (true, st) or ([[b ]]B) ∈ (false, st). *)
+      (* The first case follows trivially. *)
+      assumption.
+    + (* In the second case, [[b ]]B ∈ (false, st) contradicts our assumption that
+         [[b]]B ⊆ [[<{ true }>]]B  *)
+      destruct Hb.
+      simpl in H1.
+      apply H1 in H.
+      In_inversion.
+  - (* In the other direction, We need to show that (st, st') ∈ [[c1]] implies
+       (st, st') ∈ [[<{ if b then c1 else c2 end }>]].
+
+      Here, it suffices to show that
+      (st, st') ∈ {{(st0, st'0) | (true, st0) ∈ [[b ]]B /\ (st0, st'0) ∈ [[c1]]}},
+      which follows immediately from the assumption that (st, st') ∈ [[c1]] and
+      [[<{ true }>]]B ⊆ [[b]]B.*)
+    simpl. left; split.
+    + destruct Hb as [b_sub_tre true_sub_b].
+      apply true_sub_b. simpl. In_intro.
+    + apply st_In.
+Qed.
+
+Lemma If_while_eq :
+  forall b c,
+    <{while b do c end}> ==C <{if b then (c; while b do c end) else skip end }>.
+Proof.
+  unfold com_eqv; intros.
+  eapply Same_set_trans.
+  simpl; apply LFP_unfold.
+  apply while_body_monotone.
+  simpl.
+  split; intros x In_x.
+  - In_inversion.
+    (* The denotation of [if] is built from the denotations of each branch *)
+    + right. intuition. subst.
+      reflexivity.
+    + left. intuition.
+      eexists; intuition; eassumption.
+  - In_inversion.
+    + right. eexists. intuition. eassumption.
+      apply H1.
+    + left. intuition.
+Qed.
+
+(* Finally, we can show that the denotational and big-step operational
+   semantics of Imp are equivalent:
+
+   - Our big-step operational semantics is /sound/ with respect to the
+     denotational semantics-- if a command or expression only evaluate
+     to elements of their denotation. *)
+Lemma Denotational_A_BigStep_Sound :
+  forall a st,
+    (aeval st a, st) ∈ [[a]]A.
+Proof.
+  intros;
+  induction a; simpl; try solve [constructor]; unfold In;
+  eexists _, _; repeat split; try eassumption.
+Qed.
+
+Lemma Denotational_B_BigStep_Sound :
+  forall b st,
+    (beval st b, st) ∈ [[b]]B.
+Proof.
+  induction b; simpl; intros; try solve [constructor]; unfold In.
+  - eexists (aeval st a1), (aeval st a2); intuition.
+    + apply Denotational_A_BigStep_Sound.
+    + apply Denotational_A_BigStep_Sound.
+    + rewrite H. apply PeanoNat.Nat.eqb_refl.
+    + eapply PeanoNat.Nat.eqb_eq; assumption.
+  (* Uncomment to account for larger set of boolean expressions.
+  - eexists (aeval st a1), (aeval st a2); intuition.
+    + apply Denotational_A_BigStep_Sound.
+    + apply Denotational_A_BigStep_Sound.
+    + rewrite H, PeanoNat.Nat.eqb_refl; reflexivity.
+    + apply Bool.negb_false_iff in H.
+      eapply PeanoNat.Nat.eqb_eq; assumption.
+    - eexists (aeval st a1), (aeval st a2); intuition.
+    + apply Denotational_A_BigStep_Sound.
+    + apply Denotational_A_BigStep_Sound.
+    + apply Bool.negb_true_iff.
+      apply PeanoNat.Nat.leb_gt; assumption.
+    + apply Bool.negb_true_iff in H.
+      apply PeanoNat.Nat.leb_gt; assumption. *)
+  - eexists (aeval st a1), (aeval st a2); intuition.
+    + apply Denotational_A_BigStep_Sound.
+    + apply Denotational_A_BigStep_Sound.
+    + eapply Compare_dec.leb_correct; assumption.
+    + eapply Compare_dec.leb_complete; assumption.
+  - rewrite Bool.negb_involutive. apply IHb.
+  - eexists _, _; intuition.
+    + apply IHb1.
+    + apply IHb2.
+Qed.
+
+Lemma BigStep_Denotational_Sound :
+  forall c st st',
+    st =[c]=> st' -> (st, st') ∈ [[c]].
+Proof.
+  intros.
+  induction H; simpl; try solve [econstructor]; unfold In.
+  - (* E_Ass *)
+    eexists; split; try reflexivity.
+    rewrite <- H; eapply Denotational_A_BigStep_Sound.
+  - (* E_Seq *)
+    eexists; split; try reflexivity; eassumption.
+  - (* E_IfTrue *)
+    left; subst; split; try eassumption.
+    rewrite <- H; eapply Denotational_B_BigStep_Sound.
+  - (* E_IfFalse *)
+    right; subst; split; try eassumption.
+    rewrite <- H; eapply Denotational_B_BigStep_Sound.
+  - (* E_WhileEnd *)
+    apply LFP_unfold.
+    apply while_body_monotone.
+    left.
+    intuition.
+    rewrite <- H; apply Denotational_B_BigStep_Sound.
+  - (* E_WhileLoop *)
+    apply LFP_unfold.
+    apply while_body_monotone.
+    right.
+    eexists; repeat split; try eassumption.
+    rewrite <- H; apply Denotational_B_BigStep_Sound.
+Qed.
+
+(* Similarly, our denotational semantics is adequate with respect to
+   our big-step semantics-- when executed in an initial state included
+   in the denotation of an expression or command, that expression or
+   command will evaluate to the corresponding final state in the
+   denotation. *)
+
+Lemma BigStep_A_Denotational_Adequate :
+  forall a st v,
+    (v, st) ∈ [[a]]A
+    -> v = aeval st a.
+Proof.
+  induction a; simpl; intros st v H;
+    unfold In in H; try eassumption.
+  - destruct H as [v1 [v2 [denote_a1 [denote_a2 v_eq] ] ] ]; subst.
+    apply IHa1 in denote_a1; apply IHa2 in denote_a2.
+    subst; reflexivity.
+  - destruct H as [v1 [v2 [denote_a1 [denote_a2 v_eq] ] ] ]; subst.
+    apply IHa1 in denote_a1; apply IHa2 in denote_a2.
+    subst; reflexivity.
+  - destruct H as [v1 [v2 [denote_a1 [denote_a2 v_eq] ] ] ]; subst.
+    apply IHa1 in denote_a1; apply IHa2 in denote_a2.
+    subst; reflexivity.
+Qed.
+
+Lemma BigStep_B_Denotational_Adequate :
+  forall b st v,
+    (v, st) ∈ [[b]]B
+    -> beval st b = v.
+Proof.
+  induction b; intros st v H; In_inversion.
+  - rewrite H. reflexivity.
+  - rewrite H. reflexivity.
+  - destruct H as [v1 [v2 [denote_a1 [denote_a2 v_eq] ] ] ]; subst; simpl.
+    apply BigStep_A_Denotational_Adequate in denote_a1.
+    apply BigStep_A_Denotational_Adequate in denote_a2.
+    subst.
+    destruct (Nat.eqb (aeval st a1) (aeval st a2)) eqn: ?; intuition.
+    + rewrite H; try reflexivity.
+      apply PeanoNat.Nat.eqb_eq.
+      assumption.
+    + apply EqNat.beq_nat_false in Heqb.
+      destruct v; eauto.
+  (* Uncomment to account for larger set of boolean expressions in SF. *)
+  (*- destruct H as [v1 [v2 [denote_a1 [denote_a2 v_eq] ] ] ]; subst; simpl.
+    apply BigStep_A_Denotational_Adequate in denote_a1.
+    apply BigStep_A_Denotational_Adequate in denote_a2.
+    subst.
+    destruct (Nat.eqb (aeval st a1) (aeval st a2)) eqn: ?; intuition.
+    + rewrite H; try reflexivity.
+      apply PeanoNat.Nat.eqb_eq.
+      assumption.
+    + apply EqNat.beq_nat_false in Heqb.
+      destruct v; eauto; intuition.
+  - destruct H as [v1 [v2 [denote_a1 [denote_a2 v_eq] ] ] ]; subst; simpl.
+    apply BigStep_A_Denotational_Adequate in denote_a1.
+    apply BigStep_A_Denotational_Adequate in denote_a2.
+    subst. intuition.
+    destruct (Nat.leb (aeval st a1) (aeval st a2)) eqn: ?; intuition.
+    + destruct v; eauto; intuition.
+      apply Compare_dec.leb_complete in Heqb; lia.
+    + destruct v; eauto; intuition.
+      apply Compare_dec.leb_complete_conv in Heqb; intuition. *)
+  - destruct H as [v1 [v2 [denote_a1 [denote_a2 v_eq] ] ] ]; subst; simpl.
+    apply BigStep_A_Denotational_Adequate in denote_a1.
+    apply BigStep_A_Denotational_Adequate in denote_a2.
+    subst. intuition.
+    destruct (Nat.leb (aeval st a1) (aeval st a2)) eqn: ?; intuition.
+    + rewrite H; try reflexivity.
+      apply Compare_dec.leb_complete; assumption.
+    + apply Compare_dec.leb_complete_conv in Heqb.
+      destruct v; eauto; intuition; lia.
+  - simpl in H; In_inversion.
+    simpl; rewrite IHb with (v := negb v).
+    + apply Bool.negb_involutive.
+    + apply H.
+  - simpl in *.
+    destruct H as [v1 [v2 [denote_b1 [denote_b2 v_eq] ] ] ]; subst; simpl.
+    erewrite IHb1, IHb2 by eassumption.
+    reflexivity.
+Qed.
+
+Lemma Denotational_BigStep_Adequate :
+  forall c st st',
+    (st, st') ∈ [[c]] -> st =[c]=> st'.
+Proof.
+  induction c; unfold In; simpl; intros st st' denote_c.
+  - (* skip *)
+    subst; econstructor.
+  - (* Assignment *)
+    destruct denote_c as [v [? ?] ].
+    subst; econstructor.
+    erewrite BigStep_A_Denotational_Adequate; try reflexivity; assumption.
+  - (* Sequence *)
+    destruct denote_c as [v [denote_c1 denote_c2] ].
+    subst; econstructor.
+    + apply IHc1; eassumption.
+    + apply IHc2; eassumption.
+  - (* Conditional *)
+    destruct denote_c as [ [denote_b denote_c1] | [denote_b denote_c2] ].
+    + constructor.
+      erewrite BigStep_B_Denotational_Adequate; try reflexivity; assumption.
+      apply IHc1; eassumption.
+    + apply E_IfFalse.
+      erewrite BigStep_B_Denotational_Adequate; try reflexivity; assumption.
+      apply IHc2; eassumption.
+  - apply LFP_unfold in denote_c; try apply while_body_monotone.
+    In_inversion.
+    + rewrite H0; econstructor.
+      erewrite BigStep_B_Denotational_Adequate; try reflexivity; assumption.
+    + eapply E_WhileTrue.
+      erewrite BigStep_B_Denotational_Adequate; try reflexivity; assumption.
+      apply IHc; eassumption.
+      replace x with (fst (x, st')) by reflexivity.
+      replace st' with (snd (x, st')) at 2 by reflexivity.
+      pattern (x, st').
+      (* Hmmmm... we're (almost) back to where we started! *)
+      (* Why can't we apply the Inductive Hypothesis? *)
+      eapply Ind; try eassumption.
+      generalize IHc; clear.
+      intros IHc [st'' st']
+             [ [denote_b st_eq]
+             | [st''0 [denote_b [denote_c ? ] ] ] ].
+      * subst; econstructor.
+        erewrite BigStep_B_Denotational_Adequate; try reflexivity; assumption.
+      * econstructor.
+        erewrite BigStep_B_Denotational_Adequate; try reflexivity; assumption.
+        apply IHc; eassumption.
+        apply H.
+Qed.
+
+(* We can encode the idea of 'is a subterm' using contexts-- these are
+   programs with a single hole representing where a command can be
+   plugged in:*)
+Inductive context : Set :=
+    CHole : context
+  | CSeqL : context -> com -> context
+  | CSeqR : com -> context -> context
+  | CIf_T : bexp -> context -> com -> context
+  | CIf_E : bexp -> com -> context -> context
+  | CWhile : bexp -> context -> context.
+
+(* We can define what it means to plug in a hole by defining an
+   inductive proposition. *)
+Inductive Plug : com -> context -> com -> Prop :=
+| plug_hole : forall c, Plug c CHole c
+| plug_seq_L : forall c ctx c1 c2,
+    Plug c ctx c1 ->
+    Plug c (CSeqL ctx c2) <{c1; c2}>
+| plug_seq_R : forall c ctx c1 c2,
+    Plug c ctx c2 ->
+    Plug c (CSeqR c1 ctx) <{c1; c2}>
+| plug_if_then : forall c b ctx c1 c2,
+    Plug c ctx c1 ->
+    Plug c (CIf_T b ctx c2) <{if b then c1 else c2 end}>
+| plug_if_else : forall c b ctx c1 c2,
+    Plug c ctx c2 ->
+    Plug c (CIf_E b c1 ctx) <{if b then c1 else c2 end}>
+| plug_while_body : forall c b ctx cb,
+    Plug c ctx cb ->
+    Plug c (CWhile b ctx) <{while b do cb end}>.
+
+(* We can now show that, program equivalence entails /contextual
+   equivalence/-- that is, plugging them into the same program context
+   results in equivalent programs. *)
+Lemma contextual_equivalence :
+  forall c1 c2 ctx c1' c2',
+    Plug c1 ctx c1' ->
+    Plug c2 ctx c2' ->
+    c1 ==C c2 ->
+    c1' ==C c2'.
+Proof.
+  induction ctx; intros; inversion H; inversion H0; subst.
+  - intuition.
+  - rewrite IHctx with (c1' := c3) (c2' := c6) by assumption.
+    reflexivity.
+  - rewrite IHctx with (c1' := c4) (c2' := c7) by assumption.
+    reflexivity.
+  - rewrite IHctx with (c1' := c3) (c2' := c6) by assumption.
+    reflexivity.
+  - rewrite IHctx with (c1' := c4) (c2' := c7) by assumption.
+    reflexivity.
+  - rewrite IHctx with (c1' := cb) (c2' := cb0) by assumption.
+    reflexivity.
+Qed.
+
+(* Finally, we can use our soundness and adequacy results to show
+   that contextual equivalence holds for a notion of equivalence
+   defined in terms of the operational semantics. *)
+Lemma big_step_contextual_equivalence :
+  forall c1 c2 ctx c1' c2',
+    Plug c1 ctx c1' ->
+    Plug c2 ctx c2' ->
+    (forall st st', st =[c1]=> st' <-> st =[c2]=> st') ->
+    (forall st st', st =[c1']=> st' <-> st =[c2']=> st').
+Proof.
+  split; intros.
+  - apply Denotational_BigStep_Adequate.
+    eapply (contextual_equivalence c1 c2 ctx c1' c2' H H0).
+    + split; intros ? ?; In_inversion.
+      * eapply BigStep_Denotational_Sound.
+        apply H1.
+        apply Denotational_BigStep_Adequate.
+        assumption.
+      * eapply BigStep_Denotational_Sound.
+        apply H1.
+        apply Denotational_BigStep_Adequate.
+        assumption.
+    + eapply BigStep_Denotational_Sound.
+      assumption.
+  - apply Denotational_BigStep_Adequate.
+    eapply (contextual_equivalence c1 c2 ctx c1' c2' H H0).
+    + split; intros ? ?; In_inversion.
+      * eapply BigStep_Denotational_Sound.
+        apply H1.
+        apply Denotational_BigStep_Adequate.
+        assumption.
+      * eapply BigStep_Denotational_Sound.
+        apply H1.
+        apply Denotational_BigStep_Adequate.
+        assumption.
+    + eapply BigStep_Denotational_Sound.
+      assumption.
+Qed.
