labs/Lab8Script.v
@@ -1,0 +1,893 @@
+(* Lab 8: More Proof Automation /and/ Metatheory of Hoare Logic. *)
+
+(* Tactics covered:
+   - auto
+ *)
+
+(** Our job for this lab:
+   - Explore the magical world of proof automation in more depth
+
+   - (If there's time [but there probably won't be]), look at proof of soundness and relative completeness for Hoare logic
+ *)
+
+Set Warnings "-notation-overridden,-parsing".
+From Coq Require Import Strings.String.
+From PLF Require Import Maps.
+From Coq Require Import Bool.Bool.
+From Coq Require Import Arith.Arith.
+From Coq Require Import Arith.EqNat.
+From Coq Require Import Arith.PeanoNat. Import Nat.
+From Coq Require Import Lia.
+From PLF Require Import Hoare.
+From DS Require Import Fixpoints.
+
+(** Up to now, we've used the more manual part of Coq's tactic
+    facilities.  In this Lab, we'll learn more about some of Coq's
+    powerful automation features: proof search via the [auto] tactic,
+    automated forward reasoning via the [Ltac] hypothesis matching
+    machinery, and several additional tacticals (higher-order
+    tactics).  Using these features together with Ltac's scripting
+    facilities will enable us to make our proofs startlingly short!
+    Used properly, they can also make proofs more maintainable and
+    robust to changes in underlying definitions.  A deeper treatment
+    of [auto] and [eauto] can be found in the [UseAuto] chapter in
+    _Programming Language Foundations_.
+
+    Our motivating example will be this proof, repeated with just a
+    few small changes from the [Imp] chapter.  We will simplify this
+    proof in several stages. *)
+
+Theorem ceval_deterministic: forall c st st1 st2,
+    st =[ c ]=> st1  ->
+    st =[ c ]=> st2 ->
+    st1 = st2.
+Proof.
+  intros c st st1 st2 E1 E2.
+  generalize dependent st2.
+  induction E1.
+  - (* E_Skip *) intros st2 E2. inversion E2. subst. reflexivity.
+  - (* E_Ass *) intros st2 E2. inversion E2. subst. reflexivity.
+  - (* E_Seq *)
+    intros st2 E2. inversion E2. subst.
+    rewrite (IHE1_1 st'0 H1) in *.
+    apply IHE1_2. assumption.
+  (* E_IfTrue *)
+  - intros st2 E2. inversion E2. subst.
+    + (* b evaluates to true *)
+      apply IHE1. assumption.
+    + (* b evaluates to false (contradiction) *)
+      rewrite H in H5. discriminate.
+  - (* E_IfFalse *)
+      intros st2 E2. inversion E2. subst.
+      + (* b evaluates to true (contradiction) *)
+        rewrite H in H5. discriminate.
+      + (* b evaluates to false *)
+        apply IHE1. assumption.
+  (* E_WhileFalse *)
+  - intros st2 E2. inversion E2. subst.
+    + (* b evaluates to false *)
+      reflexivity.
+    + (* b evaluates to true (contradiction) *)
+      rewrite H in H2. discriminate.
+  (* E_WhileTrue *)
+  - intros st2 E2. inversion E2. subst.
+    + (* b evaluates to false (contradiction) *)
+      rewrite H in H4. discriminate.
+    + (* b evaluates to true *)
+      rewrite (IHE1_1 st'0 H3) in *.
+      apply IHE1_2. assumption.
+Qed.
+
+(* ################################################################# *)
+(** * The [auto] Tactic *)
+
+(** Thus far, our proof scripts mostly apply relevant hypotheses or
+    lemmas by name, and one at a time. *)
+
+Example auto_example_1 : forall (P Q R: Prop),
+  (P -> Q) -> (Q -> R) -> P -> R.
+Proof.
+  intros P Q R H1 H2 H3.
+  apply H2. apply H1. apply H3.
+Qed.
+
+(** In the fourth lab, we saw how to use the ';' tactical to chain
+    together multiple tactics: *)
+  Lemma foo : forall n, Nat.leb 0 n = true.
+  Proof.
+    intros.
+    destruct n.
+    (* Leaves two subgoals, which are discharged identically...  *)
+    - (* n=0 *) simpl. reflexivity.
+    - (* n=Sn' *) simpl. reflexivity.
+  Qed.
+
+  (** We can simplify this proof using the [;] tactical: *)
+  Lemma foo' : forall n, Nat.leb 0 n = true.
+  Proof.
+    intros; destruct n; (simpl; reflexivity).
+  Qed.
+
+  Example auto_example_1' : forall (P Q R: Prop),
+      (P -> Q) -> (Q -> R) -> P -> R.
+  Proof.
+    (* WORK IN CLASS *)
+  Admitted.
+
+  (** The [auto] tactic frees us from this drudgery by _searching_ for a
+      sequence of applications that will prove the goal: *)
+  Example auto_example_1'' : forall (P Q R: Prop),
+      (P -> Q) -> (Q -> R) -> P -> R.
+  Proof.
+    auto.
+  Qed.
+
+(** The [auto] tactic solves goals that are solvable by any combination of
+     - [intros] and
+     - [apply] (of hypotheses from the local context,
+                and additional facts (hints) specified by the user.).
+
+   This is a kind of enchanced variant of [assumption],
+   which can chain together sequences of apply to solve the current goal *)
+
+(** Using [auto] is always "safe" in the sense that it will never fail
+    and will never change the proof state: either it completely solves
+    the current goal, or it does nothing. *)
+
+  Example auto_example_1''' : forall (P Q R: Prop),
+      (P -> Q) -> (Q -> R) -> P -> R /\ 5 <= 15.
+  Proof.
+    intros P Q R H1 H2 H3.
+    (* WORK IN CLASS *)
+  Admitted.
+
+(** Here is a larger example showing [auto]'s power: *)
+
+Example auto_example_2 : forall P Q R S T U : Prop,
+  (P -> Q) ->
+  (P -> R) ->
+  (T -> R) ->
+  (S -> T -> U) ->
+  ((P->Q) -> (P->S)) ->
+  T ->
+  P ->
+  U.
+Proof. auto. Qed.
+
+(** Proof search could, in principle, take an arbitrarily long time,
+    so there are limits to how far [auto] will search by default. *)
+Example auto_example_3 : forall (P Q R S T U: Prop),
+  (P -> Q) ->
+  (Q -> R) ->
+  (R -> S) ->
+  (S -> T) ->
+  (T -> U) ->
+  P ->
+  U.
+Proof.
+  (* When it cannot solve the goal, [auto] does nothing *)
+  auto.
+  (* [auto] takes an optional argument specifying how deep to search (default is 5) *)
+  auto 6.
+Qed.
+
+(** We can extend the hint database just for the purposes of one
+    application of [auto] by writing "[auto using ...]". *)
+Lemma le_antisym : forall n m: nat, (n <= m /\ m <= n) -> n = m.
+Proof. intros. lia. Qed.
+
+Example auto_example_6 : forall n m p : nat,
+  (n <= p -> (n <= m /\ m <= n)) ->
+  n <= p ->
+  n = m.
+Proof.
+  auto.
+  intros; apply le_antisym. auto.
+  Undo 1.
+  auto using le_antisym.
+Qed.
+
+(** In any given development there will probably be
+    some specific constructors and lemmas that are used very often in
+    proofs.  We can add these to the global hint database via the command
+
+    Hint Resolve T : core.
+
+    at the top level, where [T] is a top-level theorem or a
+    constructor of an inductively defined proposition (i.e., anything
+    whose type is an implication).
+
+    When searching for potential proofs of the current goal,
+    [auto] considers the hypotheses in the current context together
+    with a _hint database_ of other lemmas and constructors. *)
+
+Theorem ceval_ex: forall c1 c2 st st1 st2,
+    st =[ c1 ]=> st1  ->
+    st1 =[ c2 ]=> st2 ->
+    st =[ c1; c2  ]=> st2.
+Proof.
+  (* WORK IN CLASS *)
+Admitted.
+
+(* Some common lemmas about equality and logical operators are
+    installed in this hint database by default.*)
+Example auto_example_4 : forall P Q R : Prop,
+  Q ->
+  (Q -> R) ->
+  P \/ (Q /\ R).
+Proof.
+  auto.
+Qed.
+
+(** If we want to see which facts [auto] is using, we can use
+    [info_auto] instead. *)
+Example auto_example_4' : forall P Q R : Prop,
+  Q ->
+  (Q -> R) ->
+  P \/ (Q /\ R).
+Proof.
+  info_auto.
+Qed.
+
+(* If [auto] tried to [apply] every available fact, it would be very
+   slow indeed, so it uses several heuristics to decide what to use.
+   We can also see which lemmas / constructors [auto] will try to
+   apply to the current goal using the [Print Hint] command.  *)
+Example auto_example_5: 2 = 2.
+Proof.
+  Print Hint.
+  info_auto.
+Qed.
+
+(**  It is also sometimes necessary to add
+
+      Hint Unfold d : core.
+
+    where [d] is a defined symbol, so that [auto] knows to expand uses
+    of [d], thus enabling further possibilities for applying lemmas that
+    it knows about. *)
+
+(** It is also possible to define specialized hint databases that can
+    be activated only when needed.  See the Coq reference manual for
+    details. *)
+
+Hint Resolve le_antisym : core.
+
+Example auto_example_6' : forall n m p : nat,
+  (n<= p -> (n <= m /\ m <= n)) ->
+  n <= p ->
+  n = m.
+Proof.
+  auto. (* picks up hint from database *)
+Qed.
+
+Definition is_fortytwo x := (x = 42).
+
+Example auto_example_7: forall x,
+  (x <= 42 /\ 42 <= x) -> is_fortytwo x.
+Proof.
+  auto.  (* does nothing *)
+  (* WORK IN CLASS *)
+Abort.
+
+Hint Unfold is_fortytwo : core.
+
+Example auto_example_7' : forall x,
+  (x <= 42 /\ 42 <= x) -> is_fortytwo x.
+Proof.
+  Print Hint.
+  info_auto. (* try also: info_auto. *)
+Qed.
+
+(* As a shorthand, we can write
+
+      Hint Constructors c : core.
+
+    to tell Coq to do a [Hint Resolve] for _all_ of the constructors
+    from the inductive definition of [c]. *)
+#[local] Hint Constructors ceval : core.
+Theorem ceval_ex_2: forall st ,
+    st =[ X := 4; Y := 5  ]=> (Y !-> 5; X !-> 4; st).
+Proof.
+  intros.
+  assert (st =[ X := 4 ]=> (X !-> 4; st)) by (econstructor; reflexivity).
+  assert ((X !-> 4; st) =[ Y := 5 ]=> (Y !-> 5; X !-> 4; st)) by (econstructor; reflexivity).
+  eauto.
+Qed.
+
+Theorem ceval_ex_2': forall st ,
+    st =[ X := 4; Y := 5  ]=> (Y !-> 5; X !-> 4; st).
+Proof.
+  debug auto.
+  (* WORK IN CLASS *)
+Admitted.
+
+(** Let's take a first pass over [ceval_deterministic] to simplify the
+    proof script. *)
+
+Theorem ceval_deterministic': forall c st st1 st2,
+    st =[ c ]=> st1  ->
+    st =[ c ]=> st2 ->
+    st1 = st2.
+Proof.
+  (* Our first optimization is to observe that we did inversion on the
+     second hypothesis in every subgoal, so let's use ";" here. *)
+  intros c st st1 st2 E1 E2.
+  generalize dependent st2;
+    induction E1; intros st2 E2; inversion E2; subst; auto.
+  - (* E_Seq *)
+    rewrite (IHE1_1 st'0 H1) in *; auto.
+  - (* E_IfTrue *)
+    + (* b evaluates to false (contradiction) *)
+      rewrite H in H5. discriminate.
+  - (* E_IfFalse *)
+    + (* b evaluates to true (contradiction) *)
+      rewrite H in H5. discriminate.
+  - (* E_WhileFalse *)
+    + (* b evaluates to true (contradiction) *)
+      rewrite H in H2. discriminate.
+  (* E_WhileTrue *)
+  - (* b evaluates to false (contradiction) *)
+    rewrite H in H4. discriminate.
+  - (* b evaluates to true *)
+    rewrite (IHE1_1 st'0 H3) in *; auto.
+Qed.
+
+(* ################################################################# *)
+(** * Searching For Hypotheses *)
+
+(** The proof has become simpler, but there is still an annoying
+    amount of repetition. Let's start by tackling the contradiction
+    cases. Each of them occurs in a situation where we have both
+
+      H1: beval st b = false
+
+    and
+
+      H2: beval st b = true
+
+    as hypotheses.  The contradiction is evident, but demonstrating it
+    is a little complicated: we have to locate the two hypotheses [H1]
+    and [H2] and do a [rewrite] following by a [discriminate].  We'd
+    like to automate this process.
+
+    (In fact, Coq has a built-in tactic [congruence] that will do the
+    job in this case.  But we'll ignore the existence of this tactic
+    for now, in order to demonstrate how to build forward search
+    tactics by hand.)
+
+    As a first step, we can abstract out the piece of script in
+    question by writing a little function in Ltac. *)
+
+Ltac rwd H1 H2 := rewrite H1 in H2; discriminate.
+
+Theorem ceval_deterministic'': forall c st st1 st2,
+    st =[ c ]=> st1  ->
+    st =[ c ]=> st2 ->
+    st1 = st2.
+Proof.
+  intros c st st1 st2 E1 E2.
+  generalize dependent st2;
+  induction E1; intros st2 E2; inversion E2; subst; auto.
+  - (* E_Seq *)
+    rewrite (IHE1_1 st'0 H1) in *.
+    auto.
+  - (* E_IfTrue *)
+    + (* b evaluates to false (contradiction) *)
+      rwd H H5.
+  - (* E_IfFalse *)
+    + (* b evaluates to true (contradiction) *)
+      rwd H H5.
+  - (* E_WhileFalse *)
+    + (* b evaluates to true (contradiction) *)
+      rwd H H2.
+  (* E_WhileTrue *)
+  - (* b evaluates to false (contradiction) *)
+    rwd H H4.
+  - (* b evaluates to true *)
+    rewrite (IHE1_1 st'0 H3) in *.
+    auto.
+Qed.
+
+(** That was a bit better, but we really want Coq to discover the
+    relevant hypotheses for us.  We can do this by using the [match
+    goal] facility of Ltac. *)
+
+Ltac find_rwd :=
+  match goal with
+    H1: ?E = true,
+    H2: ?E = false
+    |- _ => rwd H1 H2
+  end.
+
+(** This [match goal] looks for two distinct hypotheses that
+    have the form of equalities, with the same arbitrary expression
+    [E] on the left and with conflicting boolean values on the right.
+    If such hypotheses are found, it binds [H1] and [H2] to their
+    names and applies the [rwd] tactic to [H1] and [H2].
+
+    Adding this tactic to the ones that we invoke in each case of the
+    induction handles all of the contradictory cases. *)
+
+Theorem ceval_deterministic''': forall c st st1 st2,
+    st =[ c ]=> st1  ->
+    st =[ c ]=> st2 ->
+    st1 = st2.
+Proof.
+  intros c st st1 st2 E1 E2.
+  generalize dependent st2;
+  induction E1; intros st2 E2; inversion E2; subst; try find_rwd; auto.
+  - (* E_Seq *)
+    rewrite (IHE1_1 st'0 H1) in *.
+    auto.
+  - (* E_WhileTrue *)
+    + (* b evaluates to true *)
+      rewrite (IHE1_1 st'0 H3) in *.
+      auto.
+Qed.
+
+(** Let's see about the remaining cases. Each of them involves
+    applying rewrting an hypothesis after feeding it with the required
+    condition. We can automate the task of finding the relevant
+    hypotheses to rewrite with. *)
+
+Ltac find_eqn :=
+  match goal with
+    H1: forall x, ?P x -> ?L = ?R,
+    H2: ?P ?X
+    |- _ => rewrite (H1 X H2) in *
+  end.
+
+(** The pattern [forall x, ?P x -> ?L = ?R] matches any hypothesis of
+    the form "for all [x], _some property of [x]_ implies _some
+    equality_."  The property of [x] is bound to the pattern variable
+    [P], and the left- and right-hand sides of the equality are bound
+    to [L] and [R].  The name of this hypothesis is bound to [H1].
+    Then the pattern [?P ?X] matches any hypothesis that provides
+    evidence that [P] holds for some concrete [X].  If both patterns
+    succeed, we apply the [rewrite] tactic (instantiating the
+    quantified [x] with [X] and providing [H2] as the required
+    evidence for [P X]) in all hypotheses and the goal. *)
+
+Theorem ceval_deterministic''''': forall c st st1 st2,
+    st =[ c ]=> st1  ->
+    st =[ c ]=> st2 ->
+    st1 = st2.
+Proof.
+  intros c st st1 st2 E1 E2.
+  generalize dependent st2;
+  induction E1; intros st2 E2; inversion E2; subst; try find_rwd;
+    try find_eqn; eauto.
+Qed.
+
+(* That was fun, but as [ceval_ex_2'] illustrated, [auto] is not a
+   magical bullet. Let's revisit an example from a couple of labs
+   ago to see how we can use some additional tacticals to help
+   automate proofs like [ceval_ex_2']. *)
+
+(* To recap everything we've seen today:
+   - [auto] : try to solve goals via a combination of [intros] and [apply],
+     leaving the goal unchanged if any subgoals remain).
+   - [auto using X, Y, Z] : consider lemmas X, Y, and Z when using [auto].
+   - [Hint Resolve X] : Add X to a database of lemmas that [auto] should consider
+   - [Hint Unfold X] : Tell [auto] to try to [unfold X] when looking at what hints to use
+   - [Hint Constructors T] : add all the constructors of to the hint database
+
+   - [Ltac foo H := ... ]: define a new tactic
+   - [match goal with ... ] : 'pattern match' on the goal to discover the
+   - tac; [tac1 | .... | tacn] : specify a tactic for each individual subgoal.
+   - first [tac1 | .... | tacn] : apply tactics in order until the first one succeeds. Fail if none do.
+   - solve [ tac ] : use tac to solve a goal, failing otherwise.
+
+*)
+
+
+(* ################################################################# *)
+(** * Partial Hoare Logic *)
+
+
+
+Section Hoare.
+
+  (* We first develop a proof theory for building up evidence of Hoare
+     triples as an inductive proposition. Following a standard
+     convention from proof theory, we denote the claims we can build
+     evidence for using these rules as |- {{P}} c {{Q}}. *)
+  Reserved Notation " |- {{ P }}  c  {{ Q }}"
+           (at level 40, c at next level).
+
+  Inductive hoare_proof : Assertion -> com -> Assertion -> Prop :=
+  | H_Skip : forall P,
+      |- {{ P }} <{skip}> {{P}}
+  | H_Asgn : forall Q V a,
+      |- {{Q[V |-> a]}} <{V := a}> {{Q}}
+  | H_Seq  : forall P c Q d R,
+      |- {{P}} c {{Q}} ->
+       |- {{Q}} d {{R}} ->
+       |- {{P}} <{c;d}> {{R}}
+  | H_If : forall P Q b c1 c2,
+       |- {{fun st => P st /\ bassn b st}} c1 {{Q}} ->
+       |- {{fun st => P st /\ ~(bassn b st)}} c2 {{Q}} ->
+       |- {{P}} <{if b then c1 else c2 end}> {{Q}}
+  | H_While : forall P b c,
+       |- {{fun st => P st /\ bassn b st}} c {{P}} ->
+       |- {{P}} <{while b do c end}> {{fun st => P st /\ ~ (bassn b st)}}
+  | H_Consequence  : forall (P Q P' Q' : Assertion) c,
+       |- {{P'}} c {{Q'}} ->
+          P ->> P' ->
+          Q' ->> Q ->
+       |- {{P}} c {{Q}}
+
+where " |- {{ P }}  c  {{ Q }}" := (hoare_proof  P c Q) : hoare_spec_scope.
+
+  (* The triples that can be proven using these rules do not
+     necessarily align with /semantically/ valid hoare triples. The
+     proofs of soundness and completeness establish they are the same.
+     Again following proof theory conventions, we denote semantically
+     valid hoare triples as |= {{P}} c {{Q}}. *)
+
+  Notation " '|=' {{ P }}  c  {{ Q }}" :=
+    (hoare_triple  P c Q) (at level 40, c at next level)
+    : hoare_spec_scope.
+
+  (* We begin by proving that our logic is sound, i.e. it can only be
+     used to prove only semantically valid Hoare triples. *)
+
+  (* The case for the [H_While] rule is the most interesting, so we
+     define a seperate lemma for it: *)
+  Lemma hoare_while : forall P b c,
+       |= {{fun st => P st /\ bassn b st}} c {{P}} ->
+       |= {{P}} <{while b do c end}> {{fun st => P st /\ ~ (bassn b st)}}.
+  Proof.
+    unfold hoare_triple.
+    intros ? ? ? ? ? ? HE ?. remember <{while b do c end}> eqn:Heq.
+    induction HE; try inversion Heq; subst.
+    - eauto.
+    - eauto.
+  Qed.
+
+  Theorem hoare_proof_sound : forall P c Q,
+      |- {{P}} c {{Q}} ->
+      |= {{P}} c {{Q}}.
+  Proof.
+    intros ? ? ? pf.
+    (* The proof of soundness is by induction on the proof tree of the
+       claim |- {{P}} c {{Q}}. *)
+    induction pf; intros st st' HE HP; eauto using hoare_while;
+      try (inversion HE; subst; eauto);
+      eapply hoare_while; eauto.
+  Qed.
+
+  (* The weakest (liberal) precondition for an assertion [Q] and
+     command [c] is the set of initial states from which [c] always
+     either fails to terminate, or ends in a final state satisfying
+     [Q].
+
+     We define a proposition, [wlp], to capture when an assertion is a
+     weakest precondition: *)
+  Definition wlp
+             (c : com)
+             (Q : Assertion)
+             (P : Assertion)
+    : Prop := forall (P' : Assertion),
+      |= {{P'}} c {{Q}}
+      -> (P' ->> P).
+
+  (* The weakest liberal precondition for the loop [while b c] and
+     postcondition [Q] needs to be entailed by a precondition that either:
+     a) causes the loop to immediately terminate in a state satisfying Q
+     b) causes the loop to terminate in a state satisfying Q after one iteration
+     c) causes the loop to terminate in a state satisfying Q after two iterations
+     ...
+     infinity) causes the loop to run forever. *)
+
+  (* [wlp_one_iter Q c b WLP G] calculates the precondition that either:
+
+     a) makes the guard [b] false and entails [Q] OR
+
+     b) makes the guard [b] true and is the weakest precondition for
+        command [c] and postcondition [G]. *)
+
+  Definition wlp_one_iter
+             (Q : Assertion)
+             (c : com)
+             (b : bexp)
+             (WLP : com -> Assertion -> Assertion)
+             (G : Assertion)
+    : Assertion :=
+    (   (~ b /\ Q)
+        \/ (b /\ WLP c G))%assertion.
+
+  (* The weakest liberal precondition for the loop [while b c] is the
+     greatest fixed point of [wlp_one_iter]. *)
+  Definition wlp_while
+  (Q : Assertion)
+  (c : com)
+  (b : bexp)
+  (WLP : com -> Assertion -> Assertion)
+    : Assertion :=
+    @GFP state (wlp_one_iter Q c b WLP).
+
+  Fixpoint wlp_gen
+           (c : com)
+           (Q : Assertion) {struct c} : Assertion :=
+    match c with
+    | <{skip}> => Q
+    | <{ x := a}> => Q [x |-> a]
+    | <{ c1; c2 }> => wlp_gen c1 (wlp_gen c2 Q)
+    | <{ if b then c1 else c2 end }> =>
+      ((b -> wlp_gen c1 Q) /\ (~ b -> wlp_gen c2 Q))%assertion
+    | <{while b do c end }> =>
+      wlp_while Q c b wlp_gen
+    end.
+
+  Lemma wlp_ex_1 : wlp_gen <{skip}> (X = 5) = (X = 5)%assertion.
+  Proof. reflexivity. Qed.
+
+  Lemma wlp_ex_2 : wlp_gen <{X := Y + Z}> (X = 5) = (Y + Z = 5)%assertion.
+  Proof. reflexivity. Qed.
+
+  Lemma wlp_ex_3 : wlp_gen <{X := Y}> (X = Y) = (Y = Y)%assertion.
+  Proof. reflexivity. Qed.
+
+  Lemma wlp_ex_5 : wlp_gen <{X := 5}> (X = 0) = (5 = 0)%assertion.
+  Proof. reflexivity. Qed.
+
+  (* In order to reason about the greatest fixpoint of [wlp_one_iter],
+     we need to prove that [wlp_gen] is monotone. *)
+  Lemma wlp_gen_is_monotone
+    : forall (c : com),
+      Monotone (wlp_gen c).
+  Proof.
+    unfold Monotone.
+    induction c; simpl; intros; eauto.
+    - (* x := a*)
+      unfold assn_sub, Subset; eauto.
+    - (* if b then c1 else c2 end *)
+      unfold assn_sub, Subset in *; intros; eauto.
+      In_inversion.
+      In_intro; split; intros; eauto.
+      eapply IHc1; eauto.
+      Hint Unfold In : core.
+      eauto.
+      eapply IHc2; eauto.
+    - (* while b do c end *)
+      unfold wlp_while, wlp_one_iter, GFP, FConsistent, Subset in *; intros.
+      In_inversion.
+      In_intro.
+      exists x0.
+      split; eauto; intros.
+      eapply H0 in H2.
+      In_inversion.
+      + In_intro; left; split; eauto.
+        eapply H; eauto.
+      + In_intro; right; split; eauto.
+  Qed.
+
+  (* Here's an example of adding the constructors of a datatype to the
+     hint database. *)
+  Hint Constructors ceval : core.
+
+  Definition wlp_gen' (c : com) (Q : Assertion) : Assertion :=
+    fun _ => True.
+
+  Lemma wlp_gen'_is_wlp
+    : forall c Q,
+      wlp c Q (wlp_gen' c Q).
+  Proof.
+    simpl.
+    unfold wlp, wlp_gen'; simpl.
+    eauto.
+  Qed.
+
+  (* The assertion produced by [wlp_gen] is always a weakest liberal
+     precondition: *)
+  Lemma wlp_gen_is_wlp
+    : forall c Q,
+      wlp c Q (wlp_gen c Q).
+  Proof.
+    unfold wlp, hoare_triple, "->>".
+    intros; assert (forall st', st =[c]=> st' -> Q st') by eauto.
+    generalize Q st H1; clear.
+    induction c; simpl; intros; eauto.
+    - (* if b then c1 else c2 *)
+      split; eauto; intros.
+      (* Could have used [intuition] instead *)
+      eapply IHc2.
+      intros; eapply H1; eapply E_IfFalse; eauto.
+      eauto using not_true_is_false.
+    - unfold wlp_while.
+      (* The principle of coinduction allows us to prove that a particular state [st]
+         is included in the greatest fixed point.
+
+        To do so, we need to identify an F-Consistent set that includes [st].
+        In this case, it will the set of states where:
+
+        a) cause [while b do c end] to loop forever
+        b) cause [while b do c end] to terminate in a final state where Q holds
+
+ *)
+      eapply CoInd with
+          (Ind := fun st =>
+                    (forall st' : state, st =[ while b do c end ]=> st' -> Q st')
+                    /\ forall (Q : Assertion) (st : state), (forall st' : state, st =[ c ]=> st' -> Q st') ->
+                                                            wlp_gen c Q st); eauto.
+      unfold FConsistent, Subset, In; simpl; intros.
+      destruct H.
+      specialize (H1 x).
+      destruct (beval x b) eqn: ?.
+      + unfold wlp_one_iter; right; eauto 6.
+      + unfold wlp_one_iter; left; eauto.
+  Qed.
+
+  (* If the guard is true, unrolling one iteration of the loop
+     produces an equivalent weakest preondition: *)
+  Lemma wlp_unroll_true :
+    forall Q c b,
+      (wlp_while Q c b wlp_gen /\ b)%assertion ->> wlp_gen <{c; while b do c end}> Q.
+  Proof.
+    unfold "->>"; simpl; intros; intuition.
+    eapply GFP_is_FConsistent in H0; unfold wlp_one_iter, In in *; intuition.
+    unfold Monotone, Subset, In; intros; intuition.
+    right.
+    intuition.
+    eapply wlp_gen_is_monotone; eassumption.
+  Qed.
+
+  (* If the guard is false, the weakest precondition of the loop is
+     the postcondition *)
+  Lemma wlp_unroll_false :
+    forall Q c b,
+      (wlp_while Q c b wlp_gen /\ ~ b)%assertion ->> Q.
+  Proof.
+    unfold "->>"; simpl; intros; intuition.
+    eapply GFP_is_FConsistent in H0; unfold wlp_one_iter, In in *; intuition.
+    unfold Monotone, Subset, In; intros. intuition.
+    right.
+    intuition.
+    eapply wlp_gen_is_monotone; eassumption.
+  Qed.
+
+  Hint Constructors hoare_proof : core.
+  Hint Unfold assert_implies : core.
+
+  (* For all postconditions [Q] and programs [c], we can build a proof
+     of  |- {wp_gen c Q} c {Q}. *)
+  Theorem wlp_is_derivable  : forall c Q,
+       |- {{wlp_gen c Q}} c {{Q}}.
+  Proof.
+    (* The proof is by induction on c. Most of the cases follow
+       immediately from the definition of wlp, which closely follows
+       the definition of the proof rules. *)
+    induction c; simpl; intros; eauto.
+    - (* if *)
+      eapply H_If.
+      + eapply H_Consequence; eauto.
+        unfold "->>"; intuition eauto.
+      + eapply H_Consequence; eauto.
+        unfold "->>"; intuition eauto.
+    -  eapply H_Consequence with (P' := wlp_while Q c b wlp_gen)
+                                (Q' := (wlp_while Q c b wlp_gen /\ ~ b)%assertion); auto.
+      + eapply H_While.
+        eapply H_Consequence with (Q' := wlp_while Q c b wlp_gen); eauto.
+        apply wlp_unroll_true.
+      + apply wlp_unroll_false.
+  Qed.
+
+  (* Let c be a command and let P and Q be assertions such that the
+     partial correctness specification {P} c {Q} is valid. *)
+  Theorem hoare_proof_complete :
+    forall P c Q,
+      |= {{P}} c {{Q}} ->
+      |- {{P}} c {{Q}}.
+  Proof.
+    intros.
+    (*By [wlp_is_derivable] we have: |- {wp_gen c Q}} c {Q} is provable. *)
+    assert (|- {{wlp_gen c Q}} c {{Q}}) by (eauto using wlp_is_derivable).
+    (*By [wlp_gen_is_wlp] and the fact that {P} c {Q} is a valid
+      triple, then P implies [wp_gen c Q]. *)
+    assert (P ->> wlp_gen c Q) by (eapply wlp_gen_is_wlp; eauto).
+    (* By combining the rule of consequence with these two facts, the
+       proof is immediate! *)
+    eapply H_Consequence; eauto.
+  Qed.
+
+Ltac verify_assn :=
+  repeat split;
+  simpl; unfold assert_implies;
+  unfold ap in *; unfold ap2 in *;
+  unfold bassn in *; unfold beval in *; unfold aeval in *;
+  unfold assn_sub; intros;
+  repeat (simpl in *;
+          rewrite t_update_eq ||
+          (try rewrite t_update_neq; [| (intro X; inversion X; fail)]));
+  simpl in *;
+  repeat match goal with [H : _ /\ _ |- _] => destruct H end;
+  repeat rewrite not_true_iff_false in *;
+  repeat rewrite not_false_iff_true in *;
+  repeat rewrite negb_true_iff in *;
+  repeat rewrite negb_false_iff in *;
+  repeat rewrite eqb_eq in *;
+  repeat rewrite eqb_neq in *;
+  repeat rewrite leb_iff in *;
+  repeat rewrite leb_iff_conv in *;
+  try subst;
+  simpl in *;
+  repeat
+    match goal with
+      [st : state |- _] =>
+        match goal with
+        | [H : st _ = _ |- _] => rewrite -> H in *; clear H
+        | [H : _ = st _ |- _] => rewrite <- H in *; clear H
+        end
+    end;
+  try eauto; try lia.
+
+Ltac verify_ht :=
+  match goal with
+    | |- {{?P}} ?p {{?Q}} =>
+    eapply hoare_proof_sound;
+    eapply H_Consequence with (Q' := Q);
+    [ eapply wlp_is_derivable
+      | verify_assn
+      | eauto]
+  end.
+
+  Definition Hoare_Triple_1 : Prop := {{True}} <{X := 5}> {{X = 5}}.
+  Definition Hoare_Triple_2 : Prop := {{X = 2}} <{X := X + 1}> {{X = 3}}.
+  Definition Hoare_Triple_3 : Prop := {{True}} <{X := 5; Y := 0}> {{X = 5}}.
+  Definition Hoare_Triple_4 : Prop := {{X = 2 /\ X = 3}} <{X := 5}> {{X = 0}}.
+  Definition Hoare_Triple_5 : Prop :=
+    {{X = 0}}
+    <{while X = 0 do X := X + 1 end}>
+    {{X = 1}}.
+
+  Lemma Hoare_Triple_ex_1' : Hoare_Triple_1.
+  Proof.
+    unfold Hoare_Triple_1.
+    verify_ht.
+  Qed.
+
+  (* And here: *)
+  Lemma Hoare_Triple_ex_2' : Hoare_Triple_2.
+  Proof.
+    unfold Hoare_Triple_2.
+    verify_ht.
+  Qed.
+
+  (* Here is the if example from class: *)
+  Lemma Guarded_update_ex :
+  {{True}}
+  <{if (X = 0)
+    then Y := 2
+    else Y := X + 1; Y := Y + 1
+    end}>
+  {{X <= Y}}.
+  Proof.
+    verify_ht.
+  Qed.
+
+  Definition reduce_to_zero' : com :=
+    <{ while ~(X = 0) do
+               X := X - 1
+               end }>.
+
+  (* Actually proving the wlp for programs with loops amounts to
+     figuring out the right invariant! *)
+  Theorem reduce_to_zero_correct' :
+    {{True}}
+      reduce_to_zero'
+      {{X = 0}}.
+  Proof.
+    verify_ht.
+    unfold wlp_while.
+    eapply CoInd with (Ind := fun _ => True); eauto.
+    unfold FConsistent; intros ? ?.
+    In_intro.
+    unfold wlp_one_iter; intuition.
+    simpl.
+    destruct ((x X =? 0)) eqn: ?; simpl; intuition.
+    left; verify_assn.
+  Qed.
+
+End Hoare.
